ironfleet/src/Dafny/Distributed/Protocol/LiveSHT/RefinementProof/SchedulerRefinement.i.dfy
@@ -13,17 +13,12 @@ function AddPacketSets<Packet>(ps:seq<set<Packet>>) : set<Packet>
     if |ps| == 0 then {} else ps[0] + AddPacketSets(ps[1..])
 }
 
-predicate IsHostRefinementSequenceOf(hosts:seq<Host>, sends_by_step:seq<set<Packet>>, host:Host, host':Host,
-                                        receives:set<Packet>, sends:set<Packet>)
+predicate HostNextOrStutter(host:Host, host':Host, receives:set<Packet>, sends:set<Packet>)
 {
-       |hosts| > 0
-    && |sends_by_step| == |hosts| - 1
-    && host == hosts[0]
-    && host' == hosts[|hosts|-1]
-    && sends == AddPacketSets(sends_by_step)
-    && (forall p :: p in receives ==> p.dst == host.me)
-    && (forall p :: p in sends ==> p.src == host.me)
-    && (forall i :: 0 <= i < |hosts|-1 ==> Host_Next(hosts[i], hosts[i+1], receives, sends_by_step[i]))
+       (host == host' && sends == {})
+    || (   (forall p :: p in receives ==> p.dst == host.me)
+        && (forall p :: p in sends ==> p.src == host.me)
+        && Host_Next(host, host', receives, sends))
 }
 
 
@@ -40,35 +35,11 @@ lemma Lemma_HostRefinementForPacketsAppliesToIos(
     requires environment.nextStep == LEnvStepHostIos(host.me, ios);
     requires receives <= PacketsTo(LSHTEnvironment_Refine(environment), host.me);
     requires sends == LSHTPacketSet_Refine(set io | io in ios && io.LIoOpSend? :: io.s);
-    requires exists replicas, sends_at_step ::
-                 IsHostRefinementSequenceOf(replicas, sends_at_step, host, host', receives, sends);
-    ensures  exists replicas, sends_at_step ::
-                 IsHostRefinementSequenceOf(replicas, sends_at_step, host, host',
-                                               PacketsTo(LSHTEnvironment_Refine(environment), host.me), LSHTIoSeq_RefineAsSends(ios));
+    requires Host_Next(host, host', receives, sends);
+    ensures  Host_Next(host, host', PacketsTo(LSHTEnvironment_Refine(environment), host.me), LSHTIoSeq_RefineAsSends(ios));
 {
-    var hosts, sends_at_step :| IsHostRefinementSequenceOf(hosts, sends_at_step, host, host', receives, sends);
-    assert IsHostRefinementSequenceOf(hosts, sends_at_step, host, host',
-                                         PacketsTo(LSHTEnvironment_Refine(environment), host.me), LSHTIoSeq_RefineAsSends(ios));
-}
-
-lemma Lemma_LHostUnchangedImpliesExistsRefinementSequence(
-    l_host:Host,
-    l_host':Host,
-    receives:set<Packet>,
-    sends:set<Packet>
-    )
-    requires l_host == l_host';
-    requires forall p :: p in receives ==> p.dst == l_host.me;
-    requires sends == {};
-    ensures  exists h_replicas, h_sent_packets ::
-                 IsHostRefinementSequenceOf(h_replicas, h_sent_packets, l_host, l_host', receives, sends);
-{
-    var h_host := l_host;
-    var h_host' := l_host';
-
-    var h_hosts := [ h_host ];
-    var sends_by_step:seq<set<Packet>> := [];
-    assert IsHostRefinementSequenceOf(h_hosts, sends_by_step, h_host, h_host', receives, sends);
+    assert receives <= PacketsTo(LSHTEnvironment_Refine(environment), host.me);
+    assert sends == LSHTIoSeq_RefineAsSends(ios);
 }
 
 predicate LScheduler_RefinementInvariant(s:LScheduler)
