ironfleet/src/Dafny/Distributed/Common/Framework/Main.s.dfy
@@ -49,43 +49,13 @@ abstract module Main_s {
         }
     }
 
-    /*
-    lemma RefinementProof(config:ConcreteConfiguration, db:seq<DS_State>) returns (sb:seq<seq<<ServiceState>>)
-        requires |db| > 0;
-        requires DS_Init(db[0], config);
-        requires forall i :: 0 <= i < |db| - 1 ==> DS_Next(db[i], db[i+1]);
-        ensures  |sb| == |db|;
-        ensures  forall i :: 0 <= i < |sb| ==> |sb[i]| >= 1;
-        ensures  Service_Init(sb[0][0]);
-        ensures  forall i :: 0 <= i < |sb| - 1 ==> last(sb[i]) == sb[i+1][0];
-        ensures  forall i,j :: 0 <= i < |sb| && 0 <= j < |sb[i]| - 1 ==> Service_Next(sb[i][j], sb[i][j+1]);
-        ensures  forall i :: 0 <= i < |sb| ==> Service_Correspondence(db[i].environment.sentPackets, sb[i][0]);
-    */
-
-    lemma RefinementProof(config:ConcreteConfiguration, db:seq<DS_State>) returns (sb:seq<ServiceState>, cm:seq<int>)
+    lemma RefinementProof(config:ConcreteConfiguration, db:seq<DS_State>) returns (sb:seq<ServiceState>)
         requires |db| > 0;
         requires DS_Init(db[0], config);
         requires forall i {:trigger DS_Next(db[i], db[i+1])} :: 0 <= i < |db| - 1 ==> DS_Next(db[i], db[i+1]);
-        ensures  |db| == |cm|;
-        ensures  cm[0] == 0;                                            // Beginnings match
-        ensures  forall i :: 0 <= i < |cm| ==> 0 <= cm[i] < |sb|;       // Mappings are in bounds
-        ensures  forall i {:trigger cm[i], cm[i+1]} :: 0 <= i < |cm| - 1 ==> cm[i] <= cm[i+1];    // Mapping is monotonic
+        ensures  |db| == |sb|;
         ensures  Service_Init(sb[0], Collections__Maps2_s.mapdomain(db[0].servers));
-        ensures  forall i {:trigger Service_Next(sb[i], sb[i+1])} :: 0 <= i < |sb| - 1 ==> Service_Next(sb[i], sb[i+1]);
-        ensures  forall i :: 0 <= i < |db| ==> Service_Correspondence(db[i].environment.sentPackets, sb[cm[i]]);
-
-
-    /*
-    lemma DistributedSystemRefinesSpec_Init(s:DS_State, config:ProtocolConfiguration)
-        requires DS_Init(s, config);
-        requires ProtocolConfigurationInit(config, mapdomain(s.servers), s.clients);
-        ensures  Spec_Init(DS_AbstractState(s), DS_AbstractConfig(config));
-
-      // Still needs some work to talk about ios
-
-//    lemma DistributedSystemRefinesSpec_Next(s:DS_State, s':DS_State)
-//        requires DS_Next(s, s');
-//        ensures  exists states :: IsAbstractStateAbstractionSequenceOf(states, DS_AbstractState(s), DS_AbstractState(s'));
-*/
+        ensures  forall i {:trigger Service_Next(sb[i], sb[i+1])} :: 0 <= i < |sb| - 1 ==> sb[i] == sb[i+1] || Service_Next(sb[i], sb[i+1]);
+        ensures  forall i :: 0 <= i < |db| ==> Service_Correspondence(db[i].environment.sentPackets, sb[i]);
 
 }
