ironfleet/src/Dafny/Distributed/Protocol/LiveSHT/RefinementProof/SHTLemmas.i.dfy
@@ -14,85 +14,11 @@ import opened LiveSHT__SchedulerLemmas_i
 import opened LiveSHT__EnvironmentLemmas_i
 import opened LiveSHT__SHT_i
 
-function CreateSHTStateRefinementSequenceFrom(
-    ps:SHT_State,
-    actor:NodeIdentity,
-    hosts:seq<Host>,
-    sends_by_step:seq<set<Packet>>
-    ):seq<SHT_State>
-    requires |sends_by_step| == |hosts| - 1;
-    ensures  var s := CreateSHTStateRefinementSequenceFrom(ps, actor, hosts, sends_by_step);
-                |s| == |hosts|
-             && (forall i :: 0 <= i < |s| ==> s[i].config == ps.config)
-             && (forall i :: 0 <= i < |s| ==> s[i].hosts == ps.hosts[actor := hosts[i]])
-             && (forall i :: 0 <= i < |sends_by_step| ==> s[i+1].network == s[i].network + sends_by_step[i])
-             && (forall i :: 0 <= i < |sends_by_step| ==> ps.network <= s[i].network)
-             && s[0].network == ps.network
-             && s[|s|-1].network == s[0].network + AddPacketSets(sends_by_step);
-    decreases |hosts|;
-{
-    if |hosts| == 0 then
-        []
-    else if |hosts| == 1 then
-        assert |sends_by_step| == 0;
-        [ps[hosts := ps.hosts[actor := hosts[0]]]]
-    else
-        [ps[hosts := ps.hosts[actor := hosts[0]]]] + CreateSHTStateRefinementSequenceFrom(ps[network := ps.network + sends_by_step[0]], actor, hosts[1..], sends_by_step[1..])
-}
-
 lemma Lemma_HostNextImpliesHostNextWithBiggerReceiveSet(s:Host, s':Host, recvs1:set<Packet>, recvs2:set<Packet>, out:set<Packet>)
     requires Host_Next(s, s', recvs1, out);
     requires recvs1 <= recvs2;
     ensures  Host_Next(s, s', recvs1, out);
 {
-}
-
-lemma {:timeLimitMultiplier 4} Lemma_CreatingSHTStateRefinementSequenceWorks(
-    ps:SHT_State,
-    ps':SHT_State,
-    actor:NodeIdentity,
-    hosts:seq<Host>,
-    sends_by_step:seq<set<Packet>>,
-    s:seq<SHT_State>,
-    receives:set<Packet>,
-    sends:set<Packet>
-    )
-    requires |sends_by_step| == |hosts| - 1;
-    requires s == CreateSHTStateRefinementSequenceFrom(ps, actor, hosts, sends_by_step);
-    requires actor in ps.hosts;
-    requires actor in ps'.hosts;
-    requires forall id :: id in ps.hosts <==> id in ps'.hosts;
-    requires forall id :: id in ps.hosts <==> id in ps.config.hostIds;
-    requires forall oid :: oid in ps.config.hostIds && oid != actor ==> ps'.hosts[oid] == ps.hosts[oid];
-    requires ps'.hosts == ps.hosts[actor := ps'.hosts[actor]];
-    requires ps'.network == ps.network + sends;
-    requires actor in ps.config.hostIds;
-    requires SHT_MapsComplete(ps);
-    requires SHT_MapsComplete(ps');
-    requires ps.config == ps'.config;
-    requires forall p :: p in sends ==> p.src == actor;
-    requires receives <= PacketsTo(ps.network, actor);
-    requires IsHostRefinementSequenceOf(hosts, sends_by_step, ps.hosts[actor], ps'.hosts[actor], receives, sends);
-    requires sends == AddPacketSets(sends_by_step);
-    ensures  IsSHTStateRefinementSequenceOf(s, ps, ps');
-{
-    assert s[0].hosts == ps.hosts;
-    assert s[0] == ps;
-    assert s[|s|-1].hosts == ps'.hosts;
-    assert s[|s|-1] == ps';
-    
-    forall i | 0 <= i < |hosts|-1
-         ensures SHT_MapsComplete(s[i+1]);
-         ensures SHT_MapsComplete(s[i]);
-         ensures SHT_Next(s[i], s[i+1]);
-    {
-         assert receives <= PacketsTo(ps.network, actor) <= PacketsTo(s[i].network, actor);
-         assert Host_Next(hosts[i], hosts[i+1], receives, sends_by_step[i]);
-         Lemma_HostNextImpliesHostNextWithBiggerReceiveSet(hosts[i], hosts[i+1], receives, PacketsTo(s[i].network, actor), sends_by_step[i]);
-         assert Host_Next(hosts[i], hosts[i+1], PacketsTo(s[i].network, actor), sends_by_step[i]);
-         assert SHT_NextPred(s[i], s[i+1], actor, PacketsTo(s[i].network, actor), sends_by_step[i]);
-         assert SHT_Next(s[i], s[i+1]);
-    }
 }
 
 lemma {:timeLimitMultiplier 2} Lemma_HostRefinementAllowsSHTStateRefinement(
@@ -116,20 +42,31 @@ lemma {:timeLimitMultiplier 2} Lemma_HostRefinementAllowsSHTStateRefinement(
     requires actor in ps.config.hostIds;
     requires ps.network == LSHTEnvironment_Refine(environment);
     requires ps'.network == LSHTEnvironment_Refine(environment');
-    requires exists hosts, sends_by_step ::
-                 IsHostRefinementSequenceOf(hosts, sends_by_step, ps.hosts[actor], ps'.hosts[actor],
-                                               PacketsTo(LSHTEnvironment_Refine(environment), actor), LSHTIoSeq_RefineAsSends(ios));
-    ensures  exists s:seq<SHT_State> :: IsSHTStateRefinementSequenceOf(s, ps, ps');
+    requires HostNextOrStutter(ps.hosts[actor], ps'.hosts[actor],
+                               PacketsTo(LSHTEnvironment_Refine(environment), actor), LSHTIoSeq_RefineAsSends(ios));
+    ensures  SHTNextOrStutter(ps, ps');
 {
     var receives := PacketsTo(LSHTEnvironment_Refine(environment), actor);
     var sends := LSHTIoSeq_RefineAsSends(ios);
     var host := ps.hosts[actor];
     var host' := ps'.hosts[actor];
-    var hosts, sends_by_step :| IsHostRefinementSequenceOf(hosts, sends_by_step, host, host', receives, sends);
-    var s := CreateSHTStateRefinementSequenceFrom(ps, actor, hosts, sends_by_step);
+
     Lemma_EffectOnLSHTEnvironmentRefinementOfAddingPackets(environment, environment', ios);
-    Lemma_CreatingSHTStateRefinementSequenceWorks(ps, ps', actor, hosts, sends_by_step, s, receives, sends);
-    assert IsSHTStateRefinementSequenceOf(s, ps, ps');
+
+    if host' == host && sends == {} {
+        assert ps'.network == ps.network;
+        assert ps'.hosts == ps.hosts;
+        assert ps' == ps;
+        return;
+    }
+
+    assert receives <= PacketsTo(ps.network, actor);
+    assert Host_Next(host, host', receives, sends);
+    Lemma_HostNextImpliesHostNextWithBiggerReceiveSet(host, host', receives, PacketsTo(ps.network, actor), sends);
+    assert Host_Next(host, host', PacketsTo(ps.network, actor), sends);
+    assert SHT_NextPred(ps, ps', actor, PacketsTo(ps.network, actor), sends);
+    assert SHT_Next(ps, ps');
+    assert SHTNextOrStutter(ps, ps');
 }
 
 lemma Lemma_LSHTInitImpliesSHTInit(l_config:SHTConfiguration, l_ps:LSHT_State)
@@ -156,50 +93,6 @@ lemma Lemma_LSHTNextPreservesLocalInvariant(ps:LSHT_State, ps':LSHT_State)
 {
 }
 
-function CombineIntoSHTState(baseline:SHT_State, host:NodeIdentity, hosts:seq<Host>, networks:seq<Network>) : seq<SHT_State>
-    requires |hosts| == |networks|;
-    ensures  var states := CombineIntoSHTState(baseline, host, hosts, networks);
-                |states| == |hosts|
-             && forall i :: 0 <= i < |hosts| ==> states[i] == SHT_State(baseline.config, networks[i], baseline.hosts[host := hosts[i]]);
-{
-    if |hosts| == 0 then
-        []
-    else
-        [baseline[hosts := baseline.hosts[host := hosts[0]]][network := networks[0]]] + CombineIntoSHTState(baseline, host, hosts[1..], networks[1..])
-}
-
-lemma Lemma_ChangingOneHostToItselfIsNoChange(hosts:map<NodeIdentity, Host>, hosts':map<NodeIdentity, Host>, id:NodeIdentity)
-    requires id in hosts;
-    requires hosts' == hosts[id := hosts[id]];
-    ensures  hosts' == hosts;
-{
-}
-
-lemma Lemma_LeavingMostHostsUnchangedEquivalentToUpdate(hosts:map<NodeIdentity, Host>, hosts':map<NodeIdentity, Host>, id:NodeIdentity)
-    requires id in hosts && id in hosts';
-    requires forall id :: id in hosts <==> id in hosts';
-    requires forall oid :: oid in hosts && oid != id ==> oid in hosts' && hosts'[oid]==hosts[oid];
-    ensures  hosts' == hosts[id := hosts'[id]];
-{
-    var r := hosts[id := hosts'[id]];
-    forall host
-        ensures host in hosts' <==> host in r;
-        ensures host in hosts' || host in r ==> r[host] == hosts'[host];
-    {
-        if host in hosts'
-        {
-            assert host in mapdomain(hosts');
-            assert host in mapdomain(hosts);
-            assert host in r;
-        }
-        if host in r
-        {
-            assert host in hosts';
-        }
-    }
-    assert r == hosts';
-}
-
 lemma Lemma_SHTStateRefinementLeavesHostDomainUnchanged(l_ps:LSHT_State, h_ps:SHT_State)
     requires LSHTState_RefinementInvariant(l_ps);
     requires h_ps == LSHTState_Refine(l_ps);
@@ -219,16 +112,15 @@ lemma Lemma_LSHTNextOneHostMaintainsInvariant(l_s:LSHT_State, l_s':LSHT_State, i
     ensures  LSHTState_RefinementInvariant(l_s');
 {
     Lemma_LSHTNextPreservesLocalInvariant(l_s, l_s');
-    Lemma_LSchedulerNextImpliesExistsHostRefinementSequence(l_s.hosts[idx], l_s'.hosts[idx], l_s.environment, l_s'.environment, ios);
+    Lemma_LSchedulerNextImpliesHostNextOrStutter(l_s.hosts[idx], l_s'.hosts[idx], l_s.environment, l_s'.environment, ios);
 }
 
 lemma Lemma_LSHTNextOneHostImpliesSHTNext(l_ps:LSHT_State, l_ps':LSHT_State, idx:int, ios:seq<LSHTIo>)
     requires LSHT_NextOneHost(l_ps, l_ps', idx, ios);
     requires LSHTState_RefinementInvariant(l_ps);
     ensures  LSHTState_RefinementInvariant(l_ps');
-    ensures  exists s:seq<SHT_State> :: IsSHTStateRefinementSequenceOf(s, LSHTState_Refine(l_ps), LSHTState_Refine(l_ps'));
+    ensures  SHTNextOrStutter(LSHTState_Refine(l_ps), LSHTState_Refine(l_ps'));
 {
-    
     var h_ps := LSHTState_Refine(l_ps);
 
     Lemma_LSHTNextOneHostMaintainsInvariant(l_ps, l_ps', idx, ios);
@@ -246,34 +138,26 @@ lemma Lemma_LSHTNextOneHostImpliesSHTNext(l_ps:LSHT_State, l_ps':LSHT_State, idx
     {
         assert oid in mapdomain(h_ps.hosts);
         assert oid in mapdomain(h_ps'.hosts);
-        var idx := GetHostIndex(oid, l_ps.config);
+        var idx' := GetHostIndex(oid, l_ps.config);
         calc {
             h_ps.hosts[oid];
-            (l_ps.hosts[idx].host);
-            (l_ps'.hosts[idx].host);
+            (l_ps.hosts[idx'].host);
+            (l_ps'.hosts[idx'].host);
             h_ps'.hosts[oid];
         }
     }
     
-    Lemma_LSchedulerNextImpliesExistsHostRefinementSequence(l_ps.hosts[idx], l_ps'.hosts[idx], l_ps.environment, l_ps'.environment, ios);
-
+    Lemma_LSchedulerNextImpliesHostNextOrStutter(l_ps.hosts[idx], l_ps'.hosts[idx], l_ps.environment, l_ps'.environment, ios);
 
     Lemma_GetHostIndexIsUnique(l_ps.config, idx);
-    assert exists hosts, sends_by_step :: IsHostRefinementSequenceOf(hosts, sends_by_step,
-                                                                           h_ps.hosts[id], h_ps'.hosts[id],
-                                                                           PacketsTo(LSHTEnvironment_Refine(l_ps.environment), id), LSHTIoSeq_RefineAsSends(ios));
-    var hosts, sends_by_step :| IsHostRefinementSequenceOf(hosts, sends_by_step,
-                                                                 h_ps.hosts[id], h_ps'.hosts[id],
-                                                                 PacketsTo(LSHTEnvironment_Refine(l_ps.environment), id), LSHTIoSeq_RefineAsSends(ios));
     Lemma_HostRefinementAllowsSHTStateRefinement(h_ps, h_ps', id, l_ps.environment, l_ps'.environment, ios);
 }
-
 
 lemma Lemma_LSHTNextExternalImpliesSHTNext(l_ps:LSHT_State, l_ps':LSHT_State, idx:EndPoint, ios:seq<LSHTIo>)
     requires LSHT_NextExternal(l_ps, l_ps', idx, ios);
     requires LSHTState_RefinementInvariant(l_ps);
     ensures  LSHTState_RefinementInvariant(l_ps');
-    ensures  exists s:seq<SHT_State> :: IsSHTStateRefinementSequenceOf(s, LSHTState_Refine(l_ps), LSHTState_Refine(l_ps'));
+    ensures  SHTNextOrStutter(LSHTState_Refine(l_ps), LSHTState_Refine(l_ps'));
 {
     var h_ps := LSHTState_Refine(l_ps);
     //Lemma_LSHTNextOneHostMaintainsInvariant(l_ps, l_ps', idx, ios);
@@ -285,14 +169,14 @@ lemma Lemma_LSHTNextExternalImpliesSHTNext(l_ps:LSHT_State, l_ps':LSHT_State, id
     
     var s := [h_ps, h_ps'];
     assert SHT_NextExternal(h_ps, h_ps', idx, LSHTIoSeq_RefineAsSends(ios), LSHTIoSeq_RefineAsSends(ios));  // OBSERVE: exists
-    assert IsSHTStateRefinementSequenceOf(s, h_ps, h_ps');
+    assert SHTNextOrStutter(h_ps, h_ps');
 }
 
 lemma Lemma_LSHTNextEnvironmentImpliesSHTNext(l_s:LSHT_State, l_s':LSHT_State)
     requires LSHT_NextEnvironment(l_s, l_s');
     requires LSHTState_RefinementInvariant(l_s);
     requires LSHTState_RefinementInvariant(l_s');
-    ensures  exists s:seq<SHT_State> :: IsSHTStateRefinementSequenceOf(s, LSHTState_Refine(l_s), LSHTState_Refine(l_s'));
+    ensures  SHTNextOrStutter(LSHTState_Refine(l_s), LSHTState_Refine(l_s'));
 {
     var h_s := LSHTState_Refine(l_s);
     var h_s' := LSHTState_Refine(l_s');
@@ -304,14 +188,14 @@ lemma Lemma_LSHTNextEnvironmentImpliesSHTNext(l_s:LSHT_State, l_s':LSHT_State)
 
     assert h_s'.network == h_s.network;
     
-    assert IsSHTStateRefinementSequenceOf(s, LSHTState_Refine(l_s), LSHTState_Refine(l_s'));
+    assert SHTNextOrStutter(LSHTState_Refine(l_s), LSHTState_Refine(l_s'));
 }
 
 lemma Lemma_LSHTNextImpliesSHTNext(l_s:LSHT_State, l_s':LSHT_State)
     requires LSHT_Next(l_s, l_s');
     requires LSHTState_RefinementInvariant(l_s);
     ensures  LSHTState_RefinementInvariant(l_s');
-    ensures  exists s:seq<SHT_State> :: IsSHTStateRefinementSequenceOf(s, LSHTState_Refine(l_s), LSHTState_Refine(l_s'));
+    ensures  SHTNextOrStutter(LSHTState_Refine(l_s), LSHTState_Refine(l_s'));
 {
     if (exists idx, ios :: LSHT_NextOneHost(l_s, l_s', idx, ios)) {
         var idx, ios :| LSHT_NextOneHost(l_s, l_s', idx, ios);
@@ -323,4 +207,5 @@ lemma Lemma_LSHTNextImpliesSHTNext(l_s:LSHT_State, l_s':LSHT_State)
         Lemma_LSHTNextEnvironmentImpliesSHTNext(l_s, l_s');
     }
 }
+
 } 
