ironfleet/src/Dafny/Distributed/Protocol/LiveSHT/RefinementProof/SchedulerLemmas.i.dfy
@@ -7,7 +7,7 @@ import opened LiveSHT__SchedulerRefinement_i
 import opened LiveSHT__EnvironmentRefinement_i
 import opened LiveSHT__Environment_i
 
-lemma Lemma_LHostNextReceivePacketImpliesExistsHostRefinementSequence(
+lemma Lemma_LHostNextReceivePacketImpliesHostNextOrStutter(
     l_host:Host,
     l_host':Host,
     l_environment:LSHTEnvironment,
@@ -18,13 +18,10 @@ lemma Lemma_LHostNextReceivePacketImpliesExistsHostRefinementSequence(
     requires LEnvironment_Next(l_environment, l_environment');
     requires l_environment.nextStep == LEnvStepHostIos(l_host.me, ios);
     requires LHost_ReceivePacket_Next(l_host, l_host', ios);
-    ensures  exists h_hosts, sends_by_step ::
-                 IsHostRefinementSequenceOf(h_hosts, sends_by_step,
-                                               l_host, l_host', PacketsTo(LSHTEnvironment_Refine(l_environment), l_host.me), LSHTIoSeq_RefineAsSends(ios));
+    ensures  HostNextOrStutter(l_host, l_host', PacketsTo(LSHTEnvironment_Refine(l_environment), l_host.me), LSHTIoSeq_RefineAsSends(ios));
 {
     if (ios[0].LIoOpTimeoutReceive?) {
-        Lemma_LHostUnchangedImpliesExistsRefinementSequence(l_host, l_host', {}, {});
-        Lemma_HostRefinementForPacketsAppliesToIos(l_host, l_host', {}, {}, l_environment, l_environment', ios);
+        assert l_host == l_host';
         return;
     }
 
@@ -33,15 +30,12 @@ lemma Lemma_LHostNextReceivePacketImpliesExistsHostRefinementSequence(
     assert IsValidLIoOp(ios[0], l_host.me, l_environment);
     assert ios[0].r.dst == l_host.me;
     
-    var h_hosts := [l_host, l_host'];
     var sent_packets := ExtractSentPacketsFromIos(ios);
-    var sends_by_step := ExtractPacketsFromLSHTPackets(sent_packets);
-    
-    assert IsHostRefinementSequenceOf(h_hosts, [sends_by_step], l_host, l_host', PacketsTo(LSHTEnvironment_Refine(l_environment), l_host.me), LSHTIoSeq_RefineAsSends(ios));
+    Lemma_HostRefinementForPacketsAppliesToIos(l_host, l_host', PacketsTo(LSHTEnvironment_Refine(l_environment), l_host.me),
+                                               ExtractPacketsFromLSHTPackets(sent_packets), l_environment, l_environment', ios);
 }
 
-
-lemma Lemma_LHostNextProcessReceivedPacketImpliesExistsHostRefinementSequence(
+lemma Lemma_LHostNextProcessReceivedPacketImpliesHostNextOrStutter(
     l_host:Host,
     l_host':Host,
     l_environment:LSHTEnvironment,
@@ -53,17 +47,14 @@ lemma Lemma_LHostNextProcessReceivedPacketImpliesExistsHostRefinementSequence(
     requires LHost_ProcessReceivedPacket_Next(l_host, l_host', ios);
     requires LEnvironment_Next(l_environment, l_environment');
     requires l_environment.nextStep == LEnvStepHostIos(l_host.me, ios);
-    ensures  exists h_hosts, sends_by_step ::
-                 IsHostRefinementSequenceOf(h_hosts, sends_by_step,
-                                               l_host, l_host', PacketsTo(LSHTEnvironment_Refine(l_environment), l_host.me), LSHTIoSeq_RefineAsSends(ios));
+    ensures  HostNextOrStutter(l_host, l_host', PacketsTo(LSHTEnvironment_Refine(l_environment), l_host.me), LSHTIoSeq_RefineAsSends(ios));
 {
-    var h_hosts := [l_host, l_host'];
     var sent_packets := ExtractSentPacketsFromIos(ios);
-    var sends_by_step := ExtractPacketsFromLSHTPackets(sent_packets);
-    assert IsHostRefinementSequenceOf(h_hosts, [sends_by_step], l_host, l_host', PacketsTo(LSHTEnvironment_Refine(l_environment), l_host.me), LSHTIoSeq_RefineAsSends(ios));
+    Lemma_HostRefinementForPacketsAppliesToIos(l_host, l_host', PacketsTo(LSHTEnvironment_Refine(l_environment), l_host.me),
+                                               ExtractPacketsFromLSHTPackets(sent_packets), l_environment, l_environment', ios);
 }
 
-lemma Lemma_LHostNextSpontaneousImpliesExistsHostRefinementSequence(
+lemma Lemma_LHostNextSpontaneousImpliesHostNextOrStutter(
     l_scheduler:LScheduler, 
     l_scheduler':LScheduler,
     l_environment:LSHTEnvironment,
@@ -73,32 +64,22 @@ lemma Lemma_LHostNextSpontaneousImpliesExistsHostRefinementSequence(
     requires LHost_NoReceive_Next_Wrapper(l_scheduler, l_scheduler', ios);
     requires LEnvironment_Next(l_environment, l_environment');
     requires l_environment.nextStep == LEnvStepHostIos(l_scheduler.host.me, ios);
-    ensures  exists h_hosts, sends_by_step ::
-                 IsHostRefinementSequenceOf(h_hosts, sends_by_step,
-                                               l_scheduler.host, l_scheduler'.host,
-                                               PacketsTo(LSHTEnvironment_Refine(l_environment), l_scheduler.host.me), LSHTIoSeq_RefineAsSends(ios));
+    ensures  HostNextOrStutter(l_scheduler.host, l_scheduler'.host,
+                               PacketsTo(LSHTEnvironment_Refine(l_environment), l_scheduler.host.me), LSHTIoSeq_RefineAsSends(ios));
 {
     if (l_scheduler'.resendCount == 0) {
         var sent_packets := ExtractSentPacketsFromIos(ios);
-        var h_hosts := [l_scheduler.host, l_scheduler'.host];
-     
-        var sends_by_step := ExtractPacketsFromLSHTPackets(sent_packets);
-        assert IsHostRefinementSequenceOf(h_hosts, [sends_by_step],
-                                                   l_scheduler.host, l_scheduler'.host,
-                                                   PacketsTo(LSHTEnvironment_Refine(l_environment), l_scheduler.host.me), LSHTIoSeq_RefineAsSends(ios));
+        Lemma_HostRefinementForPacketsAppliesToIos(l_scheduler.host, l_scheduler'.host,
+                                                   PacketsTo(LSHTEnvironment_Refine(l_environment), l_scheduler.host.me),
+                                                   ExtractPacketsFromLSHTPackets(sent_packets), l_environment, l_environment', ios);
     } else {
         assert l_scheduler'.host == l_scheduler.host;
-
         assert ios == [];
-
-        assert IsHostRefinementSequenceOf([l_scheduler.host], [],
-                                          l_scheduler.host, l_scheduler'.host,
-                                          PacketsTo(LSHTEnvironment_Refine(l_environment), l_scheduler.host.me),
-                                          LSHTIoSeq_RefineAsSends(ios));
     }
 }
 
-lemma Lemma_LSchedulerNextImpliesExistsHostRefinementSequence(l_scheduler:LScheduler, l_scheduler':LScheduler, l_environment:LSHTEnvironment, l_environment':LSHTEnvironment, ios:seq<LSHTIo>)
+lemma Lemma_LSchedulerNextImpliesHostNextOrStutter(l_scheduler:LScheduler, l_scheduler':LScheduler, l_environment:LSHTEnvironment,
+                                                   l_environment':LSHTEnvironment, ios:seq<LSHTIo>)
     requires l_scheduler.host.constants == l_scheduler'.host.constants;
     requires l_scheduler.host.me == l_scheduler'.host.me;
     requires LScheduler_Next(l_scheduler, l_scheduler', ios);
@@ -106,22 +87,20 @@ lemma Lemma_LSchedulerNextImpliesExistsHostRefinementSequence(l_scheduler:LSched
     requires l_environment.nextStep == LEnvStepHostIos(l_scheduler.host.me, ios);
     requires LScheduler_RefinementInvariant(l_scheduler);
     ensures  LScheduler_RefinementInvariant(l_scheduler');
-    ensures  exists h_replicas, sends_by_step ::
-                 IsHostRefinementSequenceOf(h_replicas, sends_by_step,
-                                               l_scheduler.host, l_scheduler'.host,
-                                               PacketsTo(LSHTEnvironment_Refine(l_environment), l_scheduler.host.me), LSHTIoSeq_RefineAsSends(ios));
+    ensures  HostNextOrStutter(l_scheduler.host, l_scheduler'.host,
+                               PacketsTo(LSHTEnvironment_Refine(l_environment), l_scheduler.host.me), LSHTIoSeq_RefineAsSends(ios));
 {
     assert 0 <= l_scheduler'.nextActionIndex < LHost_NumActions();
     var l_host  := l_scheduler.host;
     var l_host' := l_scheduler'.host;
-
     
     if l_scheduler.nextActionIndex == 0 {
-        Lemma_LHostNextReceivePacketImpliesExistsHostRefinementSequence(l_host, l_host', l_environment, l_environment', ios);
+        Lemma_LHostNextReceivePacketImpliesHostNextOrStutter(l_host, l_host', l_environment, l_environment', ios);
     } else if l_scheduler.nextActionIndex == 1 {
-        Lemma_LHostNextProcessReceivedPacketImpliesExistsHostRefinementSequence(l_host, l_host', l_environment, l_environment', ios);
+        Lemma_LHostNextProcessReceivedPacketImpliesHostNextOrStutter(l_host, l_host', l_environment, l_environment', ios);
     } else if l_scheduler.nextActionIndex == 2 {
-        Lemma_LHostNextSpontaneousImpliesExistsHostRefinementSequence(l_scheduler, l_scheduler', l_environment, l_environment', ios);
+        Lemma_LHostNextSpontaneousImpliesHostNextOrStutter(l_scheduler, l_scheduler', l_environment, l_environment', ios);
     }
 }
+
 }
